Updated HHL formalization

mechanization/AutomatingHHL.thy
@@ -2,12 +2,22 @@ theory AutomatingHHL
   imports PaperResults
 begin
 
-(* transforms the syntactic assertion into a semantic one, because we don't have <\<sigma>> *)
-fun sp_assume where
+text \<open>This file contains the formal results mentioned the paper:
+\<^item> Theorem 1 from section 4.2: see theorem \<open>while_general_auto\<close> at the end of the file.
+\<^item> Lemma 1 from section 4.3: see lemma \<open>sound_framing_over\<close> at the end of the file.\<close>
+
+text \<open>Navigating the Isabelle formalization:
+\<^item> You can use the panel "Sidekick" on the right to see and navigate the structure of the file, via sections and subsections.
+\<^item> You can ctrl+click on terms to jump to their definition.
+\<^item> After jumping to another location, you can come back to the previous location by clicking the
+  green left arrow, on the right side of the menu above.\<close>
+
+text \<open>Quantified variables and quantified states are represented as de Bruijn indices (natural numbers).
+We use a list of values and a list of states to track quantified values and states, respectively.\<close>
+
+fun sp_assume :: "('a nstate \<Rightarrow> bool) \<Rightarrow> 'a list \<Rightarrow> 'a nstate list \<Rightarrow> 'a assertion \<Rightarrow> 'a nstate hyperassertion" 
+  where
   "sp_assume b vals states (AForallState A) S \<longleftrightarrow> (\<forall>\<phi>\<in>S. sp_assume b vals (\<phi> # states) A S)"
-(*
-  "sp_assume b vals states (AForallState A) S \<longleftrightarrow> (\<forall>\<phi>\<in>S. b \<phi> \<and> sp_assume b vals (\<phi> # states) A S)"
-*)
 | "sp_assume b vals states (AExistsState A) S \<longleftrightarrow> (\<exists>\<phi>. sp_assume b vals (\<phi> # states) A S \<and> (b \<phi> \<longrightarrow> \<phi> \<in> S))"
 | "sp_assume b vals states (AForall A) S \<longleftrightarrow> (\<forall>v. sp_assume b (v # vals) states A S)"
 | "sp_assume b vals states (AExists A) S \<longleftrightarrow> (\<exists>v. sp_assume b (v # vals) states A S)"
@@ -17,7 +27,7 @@ fun sp_assume where
 
 lemma sp_assume_works:
   assumes "sat_assertion vals states A S"
-  shows "sp_assume b vals states A (Set.filter b S)" (* Set.filter (bsem \<circ> snd) S *)
+  shows "sp_assume b vals states A (Set.filter b S)"
   using assms
   by (induct A arbitrary: vals states) (auto)
 
@@ -42,10 +52,7 @@ proof (induct A arbitrary: vals states S)
     then obtain n where "\<phi> \<in> S n" by blast
     then have "\<And>m. m \<ge> n \<Longrightarrow> sp_assume b vals (\<phi> # states) A (S m)"
       by (metis AForallState.prems(2) AForallState.prems(3) ascending_def sp_assume.simps(1) subset_eq)
-(*
-    moreover have "b \<phi>"
-      using AForallState.prems(3) \<open>\<phi> \<in> S n\<close> by auto
-*)
+
     let ?S = "shift_sequence S n"
 
     have "sp_assume b vals (\<phi> # states) A (\<Union> (range ?S))"
@@ -71,8 +78,7 @@ next
   then show ?case
     by (meson no_forall_state.simps(6) no_forall_state_after_existential.simps(7) up_closed_from_no_forall_state_sp_assume)
 next
-  case (AOr A1 A2)
-(* either A1 is infinitely often true, or either A2 is... *)
+  case (AOr A1 A2) \<comment> \<open>either A1 is infinitely often true, or either A2 is...\<close>
   show ?case
   proof (cases "holds_infinitely_often (sp_assume b vals states A1) S")
     case True
@@ -129,7 +135,7 @@ theorem while_general_no_index:
   assumes "\<Turnstile> {P} if_then b C {P}"
       and "\<Turnstile> {P} Assume (lnot b) {Q}"
       and "upwards_closed_no_index Q"
-    shows "\<Turnstile> {P} while_cond b C {Q}" (* should we add back the *\<forall><\<sigma>>. \<not> b(\<sigma>) *)
+    shows "\<Turnstile> {P} while_cond b C {Q}"
 proof (rule hyper_hoare_tripleI)
   fix S assume asm0: "P S"
   then have "\<And>n. P (iterate_sem n (if_then b C) S)"
@@ -145,43 +151,6 @@ proof (rule hyper_hoare_tripleI)
 qed
 
 
-(* TODO:
-Prove the rule with the transformation
-*)
-
-theorem while_general_auto:
-  assumes "\<Turnstile> {interp_assert I} if_then b C {interp_assert I}"
-      and "no_forall_state_after_existential I"
-    shows "\<Turnstile> {interp_assert I} while_cond b C { conj (sp_assume (lnot b \<circ> snd) [] [] I) (holds_forall (lnot b)) }"
-  using assms(1)
-proof (rule while_general_no_index)
-  show "upwards_closed_no_index (Logic.conj (sp_assume (lnot b \<circ> snd) [] [] I) (holds_forall (lnot b)))"
-  proof (rule upwards_closed_no_index_conj)
-    show "upwards_closed_no_index (holds_forall (lnot b))"
-      by (metis (no_types, opaque_lifting) holds_forall_def mem_simps(8) upwards_closed_no_indexI)
-    show "upwards_closed_no_index (sp_assume (lnot b \<circ> snd) [] [] I)"
-      by (simp add: assms(2) sp_assume_upwards_closed)
-  qed
-  show "\<Turnstile> {interp_assert I} Assume (lnot b) {Logic.conj (sp_assume ((lnot b) \<circ> snd) [] [] I) (holds_forall (lnot b))}"
-  proof (rule hyper_hoare_tripleI)
-    fix S assume asm0: "interp_assert I S"
-    then have "sp_assume (lnot b \<circ> snd) [] [] I (sem (Assume (lnot b)) S)"
-      by (simp add: assume_sem sp_assume_works)
-    moreover have "holds_forall (lnot b) (sem (Assume (lnot b)) S)"
-      by (simp add: assume_sem holds_forall_def)
-    ultimately show "Logic.conj (sp_assume (lnot b \<circ> snd) [] [] I) (holds_forall (lnot b)) (sem (Assume (lnot b)) S)"
-      by (simp add: conj_def)
-  qed
-qed
-
-(* TODO: prove that's is the strongest post? *)
-
-
-
-
-
-
-
 lemma while_exists_frame:
   assumes "\<And>\<phi>. \<Turnstile> { conj (P \<phi>) F } while_cond b C { Q \<phi> }"
   shows "\<Turnstile> { (\<lambda>S. (\<exists>\<phi> \<in> S. \<not> b (snd \<phi>) \<and> P \<phi> S) \<and> F S) } while_cond b C { (\<lambda>S. \<exists>\<phi> \<in> S. Q \<phi> S) }"
@@ -193,7 +162,6 @@ proof (rule hyper_hoare_tripleI)
   then show "\<exists>\<phi>\<in>sem (while_cond b C) S. Q \<phi> (sem (while_cond b C) S)"
     using asm0(1) asm0(2) false_state_in_while_cond by blast
 qed
-
 
 
 
@@ -262,411 +230,57 @@ proof (rule consequence_rule)
 qed (simp add: entails_refl)
 
 
+section \<open>Results from the Hypra paper\<close>
 
+text \<open>Theorem 1: Novel loop rule for \<open>\<forall>*\<exists>*\<close>-hyperproperties\<close>
 
-
-
-
-
-
-
-
-
-
-
-
-
-
-
-
-
-
-
-
-
-
-
-
-
-
-
-
-
-
-
-
-
-
-
-
-
-
-definition after_assume where
-  "after_assume I b S' = (\<exists>S. S' = sem (Assume (lnot b)) S \<and> I S)"
-
-lemma after_assume_same:
-  assumes "sat_assertion vals states A S"
-  shows "sp_assume (b \<circ> snd) vals states A (sem (Assume b) S)"
-  using sp_assume_works[of vals states A S] assms assume_sem[of b S] by simp
-
-(* is A stable by union? 
-No if there is \<forall>\<forall>
-low(l)
-*)
-
-definition limit_set where
-  "limit_set S = { \<sigma> |\<sigma> n. \<forall>m \<ge> n. \<sigma> \<in> S m}"
-
-lemma limit_setE:
-  "\<sigma> \<in> limit_set S \<Longrightarrow> (\<exists>n. \<forall>m \<ge> n. \<sigma> \<in> S m)"
-  by (simp add: limit_set_def)
-
-lemma limit_setI:
-  assumes "\<And>m. m \<ge> n \<Longrightarrow> \<sigma> \<in> S m"
-  shows "\<sigma> \<in> limit_set S"
-  using assms limit_set_def by force
-
-lemma equality_of_sets:
-  assumes "ascending (Set.filter b \<circ> S)"
-  shows "(\<Union>n. Set.filter b (S n)) = Set.filter b (limit_set S)" (is "?A = ?B")
-proof
-  show "?A \<subseteq> ?B"
-  proof
-    fix \<sigma> assume "\<sigma> \<in> ?A"
-    then obtain n where "\<sigma> \<in> S n" "b \<sigma>"
-      by force
-    moreover have "\<sigma> \<in> limit_set S"
-    proof (rule limit_setI)
-      fix m show "n \<le> m \<Longrightarrow> \<sigma> \<in> S m"
-        by (metis (no_types, lifting) ascending_def assms calculation(1) calculation(2) comp_apply member_filter subset_eq)
-    qed
-    ultimately show "\<sigma> \<in> ?B"
-      by auto
-  qed
-  show "?B \<subseteq> ?A"
-  proof
-    fix \<sigma> assume "\<sigma> \<in> ?B"
-    then obtain n where "b \<sigma>" "\<And>m. m \<ge> n \<Longrightarrow> \<sigma> \<in> S m"   
-      by (metis limit_setE member_filter)
-    then show "\<sigma> \<in> ?A"
-      by auto
-  qed
-qed
-
-lemma while_sem_new_limit:
-  "sem (while_cond b C) S = Set.filter (lnot b \<circ> snd) (limit_set (\<lambda>n. iterate_sem n (if_then b C) S))"
-proof -
-  have "filter_exp (lnot b) (\<Union>n. iterate_sem n (if_then b C) S) = Set.filter (lnot b \<circ> snd) (limit_set (\<lambda>n. iterate_sem n (if_then b C) S))"
-    using equality_of_sets
-    by (smt (verit, best) Sup.SUP_cong ascendingI comp_apply filter_exp_def filter_exp_union_general iterate_sem_assume_increasing)
-  then show ?thesis using sem_while_with_if by blast
-qed
-
-(* might not work for disjunctions... *)
-
-lemma new_powerful_lemma:
-  assumes "no_forall_state_after_existential A"
-      and "\<And>n. sat_assertion vals states A (S n)"
-    shows "sat_assertion vals states A (limit_set S)"
-  using assms
-proof (induct A arbitrary: vals states S)
-  case (AForallState A)
-(*
-    no_forall_state_after_existential A \<Longrightarrow> (\<And>n. sat_assertion ?vals ?states A (?S n)) \<Longrightarrow> sat_assertion ?vals ?states A (limit_set ?S)
-    no_forall_state_after_existential (AForallState A)
-    sat_assertion vals states (AForallState A) (S ?n)
-*)
-  then have "\<And>n \<phi>. \<phi> \<in> S n \<Longrightarrow> sat_assertion vals (\<phi> # states) A (S n)"
-    using sat_assertion.simps(3) by blast
-(*
-We need to shift, but maybe too much (infinitely...)
-*)
-
-  then show "sat_assertion vals states (AForallState A) (limit_set S)" sorry
-next
-  case (AExistsState A)
-(* we can shift by n *)
-  then show ?case sorry
-next
-  case (AForall A)
-  then show ?case sorry
-next
-  case (AExists A)
-(* we can shift by n *)
-  then show ?case sorry
-next
-  case (AOr A1 A2)
-(*
-At least one holds infinitely often...
-\<longrightarrow> Is the limit the same if we project? Maybe not...
-*)
-  then show ?case sorry
-qed (auto)
-
-
-lemma after_assume_same_two:
-  assumes "sp_assume (b \<circ> snd) vals states A S'"
-      and "\<forall>\<phi> \<in> S'. b (snd \<phi>)"
-(*
-And A is satisfiable... by something larger than S'?
-*)
-(* Assume A = A1 \<and> A2 *)
-(*
-A1 = \<forall><\<phi>>. \<phi>(x) = 5
-A2 = \<forall><\<phi>>. \<phi>(x) = 6
-S' would not satisfy it...
-S' would be empty
-
-*)
-
-(*
-How do I construct S?
-*)
-    shows "\<exists>S. S' = sem (Assume b) S \<and> sat_assertion vals states A S"
-  using assms
-proof (induct A arbitrary: vals states)
-  case (AConst x)
-  then show ?case
-    by (metis holds_forall_def sem_assume_low_exp(1) sp_assume.simps(7))
-next
-  case (AComp x1a x2 x3a)
-  then show ?case
-    by (metis holds_forallI sem_assume_low_exp(1) sp_assume.simps(8))
-next
-  case (AForallState A)
-  then show ?case sorry
-next
-  case (AExistsState A)
-(*
-    sp_assume (b \<circ> snd) ?vals ?states A S' \<Longrightarrow> \<forall>\<phi>\<in>S'. b (snd \<phi>) \<Longrightarrow> \<exists>S. S' = sem (Assume b) S \<and> sat_assertion ?vals ?states A S
-    sp_assume (b \<circ> snd) vals states (AExistsState A) S'
-    \<forall>\<phi>\<in>S'. b (snd \<phi>)
-*)
-  then obtain \<phi> where "sp_assume (b \<circ> snd) vals (\<phi> # states) A S'" "(b \<circ> snd) \<phi> \<Longrightarrow> \<phi> \<in> S'"
-    by (metis sp_assume.simps(2))
-
-
-
-  then show "\<exists>S. S' = sem (Assume b) S \<and> sat_assertion vals states (AExistsState A) S" sorry
-next
-  case (AForall A)
-  then show ?case sorry
-next
-  case (AAnd A1 A2)
-(*
-  then obtain S1 S2 where "S' = sem (Assume b) S1 \<and> sat_assertion vals states A1 S1"
-    "S' = sem (Assume b) S2 \<and> sat_assertion vals states A2 S2"
-    by (meson sp_assume.simps(5))
-
-*)
-
-
-  then show ?case sorry
-qed (fastforce+)
-
-
-
-
-
-
-lemma upwards_closed_before_then_after:
-  assumes "no_forall_state_after_existential I"
-  shows "upwards_closed (\<lambda>n. sp_assume b vals states I) (sp_assume b vals states I)"
-  by (simp add: assms sp_assume_upwards_closed upwards_closed_def)
-
-
-
-lemma no_forall_state_after_existential_sem_after_assume:
-  assumes "no_forall_state_after_existential I"
-      and "ascending S_not_b" (* the not_b set always increases *)
-      and "\<And>n. S_b (Suc n) = f (S_b n)" (* the b_set is a function of itself only *)
-      and "\<And>n. S_b n = Set.filter b (S n) \<and> S_not_b n = Set.filter (lnot b) (S n)" (* partition *)
-      and "\<And>n. sat_assertion vals states I (S n)"
-(* loop sem: \<Union>n. S_not_b n
-How do I express Q?
- *)
-    shows "\<exists>S_union. sat_assertion vals states I S_union \<and> (\<Union>n. S_not_b n) = Set.filter (lnot b) S_union"
-  using assms
-proof (induct I arbitrary: vals states S S_b S_not_b)
-  case (AForallState A)
-(*
-... \<Longrightarrow> \<exists>S_union. sat_assertion ?vals ?states A S_union \<and> \<Union> (range S_not_b) = Set.filter (lnot b) S_union
-    no_forall_state_after_existential (AForallState A)
-    ascending S_not_b
-    S_b (Suc ?n) = f (S_b ?n)
-    S_b ?n = Set.filter b (S ?n) \<and> S_not_b ?n = Set.filter (lnot b) (S ?n)
-    sat_assertion vals states (AForallState A) (S ?n)
-*)
-(*
-Two cases: \<phi> \<in> S_b, or \<phi> \<in> S_not_b 
-*)
-  then have "\<And>n \<phi>. \<phi> \<in> S n \<Longrightarrow> sat_assertion vals (\<phi> # states) A (S n)"
-    by simp
-  thm AForallState(1)[of _ _ _ vals "\<phi> # states"]
-(*
-\<exists>S_union. sat_assertion vals (\<phi> # states) A S_union \<and> \<Union> (range ?S_not_b) = Set.filter (lnot b) S_union
-\<longrightarrow> *one* S_union per state \<phi>
-\<longrightarrow> How do we construct the final S_union?
-*)
-
-
-  show "\<exists>S_union. sat_assertion vals states (AForallState A) S_union \<and> \<Union> (range S_not_b) = Set.filter (lnot b) S_union"
-    sorry
-  proof (rule sat_assertion_aforallstateI)
-    fix \<phi>
-    assume "\<phi> \<in> \<Union> (range S)"
-    then obtain n where "\<phi> \<in> S n" by blast
-    then have "\<And>m. m \<ge> n \<Longrightarrow> sat_assertion vals (\<phi> # states) A (S m)"
-      by (meson AForallState.prems(2) AForallState.prems(3) ascending_def sat_assertion.simps(3) subsetD)
-    let ?S = "shift_sequence S n"
-    have "sat_assertion vals (\<phi> # states) A (\<Union> (range ?S))"
-    proof (rule AForallState(1))
-      show "no_forall_state_after_existential A"
-        using AForallState.prems(1) by auto
-      show "ascending ?S"
-        by (simp add: AForallState.prems(2) shift_sequence_properties(1))
-      fix m show "sat_assertion vals (\<phi> # states) A (shift_sequence S n m)"
-        by (simp add: \<open>\<And>m. n \<le> m \<Longrightarrow> sat_assertion vals (\<phi> # states) A (S m)\<close> shift_sequence_def)
-    qed
-    then show "sat_assertion vals (\<phi> # states) A (\<Union> (range S))"
-      by (metis AForallState.prems(2) shift_sequence_properties(2))
-  qed
-next
-  case (AExistsState A)
-  then show ?case
-    by (meson no_forall_state.simps(4) no_forall_state_after_existential.simps(8) up_closed_from_no_exists_state_false)
-next
-  case (AExists A)
-  then show ?case
-    by (meson no_forall_state.simps(6) no_forall_state_after_existential.simps(7) up_closed_from_no_exists_state_false)
-next
-  case (AOr A1 A2)
-(* either A1 is infinitely often true, or either A2 is... *)
-  show ?case
-  proof (cases "holds_infinitely_often (sat_assertion vals states A1) S")
-    case True
-    then have "sat_assertion vals states A1 (\<Union> (range (subseq_sat (sat_assertion vals states A1) S)))"
-      using AOr.hyps(1) AOr.prems(1) AOr.prems(2) subseq_sat_properties(1) subseq_sat_properties(2) no_forall_state_after_existential.simps(6) by blast
-    then show ?thesis
-      using AOr.prems(2) True subseq_sat_properties(3) by fastforce
-  next
-    case False
-    then have "holds_infinitely_often (sat_assertion vals states A2) S"
-      using AOr.prems(3) sat_assertion.simps(8) holds_infinitely_often_def
-      by (metis gt_ex max_less_iff_conj)
-    then have "sat_assertion vals states A2 (\<Union> (range (subseq_sat (sat_assertion vals states A2) S)))"
-      using AOr.hyps(2) AOr.prems(1) AOr.prems(2) subseq_sat_properties(1) subseq_sat_properties(2) no_forall_state_after_existential.simps(6) by blast
-    then show ?thesis
-      using AOr.prems(2) \<open>holds_infinitely_often (sat_assertion vals states A2) S\<close> subseq_sat_properties(3) by fastforce
-  qed
-next
-  case (AAnd A1 A2)
-  then show ?case
-    using sat_assertion.simps(7) no_forall_state_after_existential.simps(5) by blast
-qed (simp_all)
-
-
-
-
-
-
-
-
-lemma sem_while_with_if_union_outside:
-  "sem (while_cond b C) S = (\<Union>n. filter_exp (lnot b) (iterate_sem n (if_then b C) S))"
-  by (simp add: filter_exp_union_general sem_while_with_if)
-
-
-lemma upwards_closed_before_then_after:
-  assumes "upwards_closed (\<lambda>n. I) I"
-  shows "upwards_closed (\<lambda>n. after_assume I b) (after_assume I b)"
-proof (rule upwards_closedI)
-  fix S' assume asm0: "ascending S'" "\<forall>n. after_assume I b (S' n)"
-  then have "\<And>n. \<exists>S. S' n = sem (Assume (lnot b)) S \<and> I S"
-    by (simp add: after_assume_def)
-  moreover obtain S where "ascending S" 
-
+text \<open>This result uses the following constructs:
+\<^item> \<^term>\<open>conj A B\<close> corresponds to the hyper-assertion \<open>A \<and> B\<close>.
+\<^item> \<^term>\<open>sp_assume (lnot b \<circ> snd) [] [] I\<close> corresponds to \<open>\<Theta>\<^sub>\<not>\<^sub>b(I)\<close>.
+\<^item> \<^term>\<open>holds_forall b\<close> corresponds to \<open>box(b)\<close>.\<close>
 
 theorem while_general_auto:
-  assumes "\<Turnstile> {I} if_then b C {I}"
-      and "upwards_closed (\<lambda>(n::nat). I) I"
-    shows "\<Turnstile> {I} while_cond b C {after_assume I b}"
-proof (rule hyper_hoare_tripleI)
-  fix S assume asm0: "I S"
-  then have "\<And>n. I (iterate_sem n (if_then b C) S)"
-    by (meson assms(1) indexed_invariant_then_power)
-  then have "\<And>n. after_assume I b (filter_exp (lnot b) (iterate_sem n (if_then b C) S))"
-    by (metis after_assume_def assume_sem filter_exp_def)
-  moreover have "ascending (\<lambda>n. filter_exp (lnot b) (iterate_sem n (if_then b C) S))"
-    by (meson ascendingI iterate_sem_assume_increasing)
-
-
-
-  then have "\<And>n. Q n (filter_exp (lnot b) (union_up_to_n (if_then b C) S n))"
-    by (metis assms(2) assume_sem filter_exp_def hyper_hoare_triple_def iterate_sem_assume_increasing_union_up_to)
-
-    by (simp add: ascending_iterate_filter)
-  ultimately have "Q_inf (sem (while_cond b C) S)"
-    by (metis (no_types, lifting) SUP_cong assms(3) filter_exp_union_general iterate_sem_assume_increasing_union_up_to sem_while_with_if upwards_closed_def)
-  then show "Logic.conj Q_inf (holds_forall (lnot b)) (sem (while_cond b C) S)"
-    by (simp add: conj_def filter_exp_def holds_forall_def sem_while_with_if)
-qed
-
-
-
-
-lemma ascending_union_up_to:
-  "ascending (\<lambda>n. union_up_to_n (if_then b C) S n)"
-  by (simp add: ascending_def union_up_to_increasing)
-
-
-
-
-fun after_assume_indexed where
-  "after_assume_indexed I b 0 S' = (\<exists>S. S' = sem (Assume (lnot b)) S \<and> I S)"
-| "after_assume_indexed I b (Suc n) S' = (\<exists>S. S' = sem (Assume (lnot b)) S \<and> I S)"
-(* needs to relate this existential to the previous one, included *)
-
-
-
-(* weird, because goes backward, not unique... will not be ascending...
-
-Can we create it?
-(* S n should become larger *)
-*)
-
-  then show "after_assume I b (\<Union> (range S'))" sorry
-qed
-
-
-lemma while_forall_exists_simpler_for_automation:
   assumes "\<Turnstile> {interp_assert I} if_then b C {interp_assert I}"
       and "no_forall_state_after_existential I"
-    shows "\<Turnstile> {interp_assert I} while_cond b C {after_assume (interp_assert I) b}"
-proof -
-  have "\<Turnstile> {interp_assert I} while_cond b C {Logic.conj (after_assume (interp_assert I) b) (holds_forall (lnot b))}"
-    using assms(1)
-  proof (rule while_general)
-(*
- 1. \<And>n. \<Turnstile> {interp_assert I} Assume (lnot b) {?Q n}
- 2. upwards_closed ?Q (after_assume (interp_assert I) b)
-*)
-    show "upwards_closed (\<lambda>n. after_assume (interp_assert I) b) (after_assume (interp_assert I) b)"
-      by (simp add: assms(2) upwards_closed_before_then_after upwards_closed_syn_sem_practical)
-    show "\<Turnstile> {interp_assert I} Assume (lnot b) {after_assume (interp_assert I) b}"
-      by (metis after_assume_def hyper_hoare_tripleI)
+    shows "\<Turnstile> {interp_assert I} while_cond b C { conj (sp_assume (lnot b \<circ> snd) [] [] I) (holds_forall (lnot b)) }"
+  using assms(1)
+proof (rule while_general_no_index)
+  show "upwards_closed_no_index (Logic.conj (sp_assume (lnot b \<circ> snd) [] [] I) (holds_forall (lnot b)))"
+  proof (rule upwards_closed_no_index_conj)
+    show "upwards_closed_no_index (holds_forall (lnot b))"
+      by (metis (no_types, opaque_lifting) holds_forall_def mem_simps(8) upwards_closed_no_indexI)
+    show "upwards_closed_no_index (sp_assume (lnot b \<circ> snd) [] [] I)"
+      by (simp add: assms(2) sp_assume_upwards_closed)
   qed
-  then show ?thesis
-    by (simp add: conj_def hyper_hoare_triple_def)
+  show "\<Turnstile> {interp_assert I} Assume (lnot b) {Logic.conj (sp_assume ((lnot b) \<circ> snd) [] [] I) (holds_forall (lnot b))}"
+  proof (rule hyper_hoare_tripleI)
+    fix S assume asm0: "interp_assert I S"
+    then have "sp_assume (lnot b \<circ> snd) [] [] I (sem (Assume (lnot b)) S)"
+      by (simp add: assume_sem sp_assume_works)
+    moreover have "holds_forall (lnot b) (sem (Assume (lnot b)) S)"
+      by (simp add: assume_sem holds_forall_def)
+    ultimately show "Logic.conj (sp_assume (lnot b \<circ> snd) [] [] I) (holds_forall (lnot b)) (sem (Assume (lnot b)) S)"
+      by (simp add: conj_def)
+  qed
 qed
 
-lemma no_forall_state_after_existential_sem:
-  assumes "no_forall_state_after_existential A"
-      and "ascending S"
-      and "\<And>n. sat_assertion vals states A (S n)"
-    shows "sat_assertion vals states A (\<Union>n. S n)"
-  using assms
+text \<open>Lemma 1.\<close>
 
+text \<open>In the formalization, states have a logical part (omitted in the paper) as well as a program part.
+Our lemma below expresses equality of the logical parts (fst), and equality of non-modified variables
+for the program part (snd).\<close>
+
+lemma sound_framing_over:
+  "\<forall>\<sigma>' \<in> sem C S. \<exists>\<sigma> \<in> S. (\<forall>x. x \<notin> wr C \<longrightarrow> snd \<sigma> x = snd \<sigma>' x) \<and> fst \<sigma> = fst \<sigma>'"
+proof clarify
+  fix l \<sigma>' assume asm0: "(l, \<sigma>') \<in> sem C S"
+  then obtain \<sigma> where "(l, \<sigma>) \<in> S" "\<langle>C, \<sigma>\<rangle> \<rightarrow> \<sigma>'"
+    by (metis in_sem prod.sel(1) prod.sel(2))
+  then have "agree_on (- wr C) \<sigma> \<sigma>'"
+    by (simp add: wr_charact)
+  then show "\<exists>\<sigma>\<in>S. (\<forall>x. x \<notin> wr C \<longrightarrow> snd \<sigma> x = snd (l, \<sigma>') x) \<and> fst \<sigma> = fst (l, \<sigma>')"
+    by (metis (mono_tags, lifting) ComplI \<open>(l, \<sigma>) \<in> S\<close> agree_onE fst_conv snd_conv)
+qed
 
 
 end
